bedrock2.Semantics: commit to little-endian

bedrock2/src/BasicC64Semantics.v
@@ -1,23 +1,8 @@
-Require Import Coq.NArith.BinNatDef.
+Require Import Coq.ZArith.ZArith.
 Require Import bedrock2.Syntax bedrock2.BasicC64Syntax bedrock2.Semantics.
 Require bedrock2.String bedrock2.Map.SortedList bedrock2.Map.SortedListString.
-Require Import coqutil.Word.Interface coqutil.Datatypes.HList coqutil.Datatypes.PrimitivePair.
+Require Import coqutil.Word.Interface.
 Require coqutil.Word.Naive.
-Import ZArith.
-Definition word := Word.Naive.word 64 (proj2 (Zlt_is_lt_bool 0 64) eq_refl).
-Definition byte := Word.Naive.word 8 (proj2 (Zlt_is_lt_bool 0 8) eq_refl).
-Definition bytes_per sz := match sz with access_size.one => 1 | access_size.two => 2 | access_size.four => 4 | access_size.word => 8 end.
-Fixpoint combine (n : nat) : forall (bs : tuple byte n), word :=
-  match n with
-  | O => fun _ => word.of_Z 0
-  | S n => fun bs => word.or (word.of_Z (word.unsigned (pair._1 bs)))
-                             (word.slu (combine n (pair._2 bs)) (word.of_Z 8))
-  end.
-Fixpoint split (n : nat) (w :word) : tuple byte n :=
-  match n with
-  | O => tt
-  | S n => pair.mk (word.of_Z (word.unsigned w)) (split n (word.sru w (word.of_Z 8)))
-  end.
 Instance parameters : parameters :=
   let word := Word.Naive.word 64 (proj2 (Zlt_is_lt_bool 0 64) eq_refl) in
   let byte := Word.Naive.word 8 (proj2 (Zlt_is_lt_bool 0 8) eq_refl) in
@@ -42,9 +27,6 @@ Instance parameters : parameters :=
   (* TODO: bedrock2.Byte, bedrock2.Word8 *)
   Semantics.byte := byte;
   mem := SortedList.map (SortedList.parameters.Build_parameters word byte word.eqb word.ltu);
-  Semantics.bytes_per := bytes_per;
-  Semantics.combine sz := combine (bytes_per sz);
-  Semantics.split sz := split (bytes_per sz);
   locals := SortedListString.map _;
   funname_eqb := String.eqb;
 |}.
