bedrock2/src/Semantics.v
@@ -1,9 +1,34 @@
 Require Import coqutil.sanity coqutil.Macros.subst coqutil.Macros.unique.
 Require Import coqutil.Datatypes.PrimitivePair coqutil.Datatypes.HList.
 Require Import bedrock2.Notations bedrock2.Syntax coqutil.Map.Interface.
-Require Import BinIntDef coqutil.Word.Interface.
+Require Import BinIntDef coqutil.Word.Interface coqutil.Word.LittleEndian.
 
 Require Coq.Lists.List.
+
+(* TODO: moveme *)
+Module List.
+  Section WithA.
+    Context {A : Type}.
+    Fixpoint option_all (xs : list (option A)) {struct xs} : option (list A) :=
+      match xs with
+      | nil => Some nil
+      | cons ox xs =>
+        match ox, option_all xs with
+        | Some x, Some ys => Some (cons x ys)
+        | _ , _ => None
+        end
+      end.
+
+    Section WithStep.
+      Context (step : A -> A).
+      Fixpoint unfoldn (n : nat) (start : A) :=
+        match n with
+        | 0%nat => nil
+        | S n => cons start (unfoldn n (step start))
+        end.
+    End WithStep.
+  End WithA.
+End List.
 
 Class parameters := {
   syntax :> Syntax.parameters;
@@ -16,43 +41,26 @@ Class parameters := {
   locals :> map.map varname word;
 
   interp_binop : bopname -> word -> word -> word;
-
-  bytes_per : access_size -> nat;
-  combine : forall sz, tuple byte (bytes_per sz) -> word;
-  split : forall sz, word -> tuple byte (bytes_per sz);
-
   funname_eqb : funname -> funname -> bool
 }.
 
 Section semantics.
   Context {pp : unique! parameters}.
+  Definition bytes_per sz :=
+    match sz with
+      | access_size.one => 1 | access_size.two => 2 | access_size.four => 4
+      | access_size.word => Z.to_nat (Z.div (Z.add width 7) 8)
+    end%nat.
 
-  Section WithMem.
-    Context (m:mem).
-    Fixpoint load_bytes (n : nat) (a : word) {struct n} : option (tuple byte n) :=
-      match n with
-      | O => Some tt
-      | S n =>
-        'Some b <- map.get m a | None;
-        'Some bs <- load_bytes n (word.add (word.of_Z 1%Z) a) | None;
-        Some (pair.mk b bs)
-      end.
-  End WithMem.
-  Definition load m a sz : option word :=
-    'Some bs <- load_bytes m (bytes_per sz) a | None;
-    Some (combine sz bs).
-  Fixpoint store_bytes (n : nat) (m:mem) (a : word) : forall (bs : tuple byte n), mem :=
-    match n with
-    | O => fun bs => m
-    | S n => fun bs => store_bytes n (map.put m a (pair._1 bs)) (word.add (word.of_Z 1%Z) a) (pair._2 bs)
-    end.
-  Definition store sz m a v : option mem :=
-    'Some _ <- load m a sz | None;
-    Some (store_bytes (bytes_per sz) m a (split sz v)).
   Definition trace := list ((mem * actname * list word) * (mem * list word)).
 
-  Context (eval : locals -> expr -> word -> Prop).
-  Context (rely guarantee : trace -> Prop) (progress : trace -> trace -> Prop).
-  Implicit Types post : trace -> mem -> locals -> Prop. (* COQBUG(unification finds Type instead of Prop and fails to downgrade *)
-
+  Definition footprint a sz := List.unfoldn (word.add (word.of_Z 1)) (bytes_per sz) a.
+  Definition load (m:mem) a sz : option word := 
+    'Some bs <- List.option_all (List.map (map.get m) (footprint a sz)) | None ;
+    Some (word.of_Z (LittleEndian.combine _ (tuple.of_list bs))).
+  Definition unchecked_store (m:mem) a sz v : option mem :=
+    map.putmany_of_list (footprint a sz) (tuple.to_list (LittleEndian.split (bytes_per sz) (word.unsigned v))) m.
+  Definition store sz m a v : option mem :=
+    'Some _ <- load m a sz | None;
+    unchecked_store m a sz v.
 End semantics.
